theories/soundness/dyn_getc.v
@@ -60,16 +60,24 @@ Section proofs.
     { iDestruct "H" as "%H".
       discriminate H.
     }
-    iDestruct "He" as (dyntag Σdyn dyndef hpure) "He".
+    iDestruct "He" as (dyntag Σdyn dyndef hpure) "[#HΣdyn He]".
     destruct hpure as [hdyndef hsupdyn].
     rewrite interp_tag_equiv; last by apply wfpdefs.
-    iDestruct "He" as (?? def def0 ????) "[%H [#hmixed [#hconstr [#hf0 [#hdyn H◯]]]]]".
+    iDestruct "He" as (?? def def0 ????) "(%H & #hmixed & #hconstr & #hf0 & #hdyn & H◯)".
     destruct H as ([= <-] & hdef & hdef0 & hlen & ? & hinherits & hfields & hidom).
     simplify_eq.
     assert (hl0: length (generics dyndef) = length σ).
     { apply inherits_using_wf in hinherits; try (by apply wfpdefs).
       destruct hinherits as (?&?&?&hh).
       inv hh; by simplify_eq.
+    }
+    pose (Δdyn0 := Δsdt def0.(generics) (gen_targs (length def0.(generics)))).
+    pose (Δdyn := Δsdt dyndef.(generics) σ).
+    assert (hnewcond: ∀ k c, Δdyn0 !! k = Some c → def0.(constraints) ++ Δdyn ⊢ c.1 <D: c.2).
+    { apply inherits_using_extends_dyn in hinherits; try by apply wfpdefs.
+      destruct hinherits as (def0' & ? & hdef0' & ? & hwf); simplify_eq.
+      move => k c hc.
+      by apply hwf with k.
     }
     iAssert (⌜t0 = t⌝ ∗ heap_models h ∗ ▷ interp_type DynamicT Σt v)%I with "[Hh]" as "[%Ht [Hh Hv]]".
     { iDestruct "Hh" as (sh) "(H● & %hdom & #Hh)".
@@ -84,7 +92,7 @@ Section proofs.
       (* the field must be public, since we can't access it from This *)
       destruct H9 as (vis & fty & orig & hf & hvc).
       destruct vis; last by destruct recv.
-      assert (hsub: def0.(constraints) ⊢ fty <D: DynamicT).
+      assert (hsub: def0.(constraints) ++ Δdyn0 ⊢ fty <D: DynamicT).
       { destruct wfpdefs.
         assert (h0 := hinherits).
         apply inherits_using_dyn_parent in h0 => //.
@@ -98,16 +106,157 @@ Section proofs.
         apply h1 in hf.
         by apply hf.
       }
+      assert (hsub' : def0.(constraints) ++ Δdyn ⊢ fty <D: DynamicT).
+      { eapply subtype_constraint_trans; first by apply hsub.
+        move => i c hc.
+        rewrite lookup_app in hc.
+        destruct (constraints def0 !! i) as [[??] | ] eqn:h0.
+        - rewrite h0 in hc; case: hc => <-.
+          eapply subtype_weaken.
+          + apply SubConstraint.
+            apply elem_of_list_lookup_2 with i.
+            by apply h0.
+          + by set_solver.
+        - rewrite h0 in hc.
+          by eapply hnewcond.
+      }
       destruct wfpdefs.
       assert (hwfc: Forall wf_constraint def0.(constraints)) by by apply wf_constraints_wf in hdef0.
-      iSpecialize ("hdyn" $! name Public fty orig hf).
+      assert (hwfd: Forall wf_constraint Δdyn).
+      { apply Δsdt_wf.
+        apply inherits_using_wf in hinherits => //.
+        destruct hinherits as (? & ? & ? & hwf); simplify_eq.
+        by apply wf_ty_class_inv in hwf.
+      }
+      assert (hwf_ : Forall wf_constraint (def0.(constraints) ++ Δdyn)).
+      { apply Forall_app; by split.
+      }
       iNext.
+      iAssert (□ Σinterp Σt Δdyn)%I as "#hconstr_dyn".
+      { iClear "Hle hmixed hconstr hdyn H◯ Hh HΦ H H▷".
+        iModIntro; iIntros (i c hc w) "#h".
+        apply Δsdt_lookup_Some in hc as (k & var & ty & hvk & htk & hk).
+        iDestruct ("HΣdyn" $! k var hvk) as (ϕ) "[hϕ hiϕ]"; iClear "HΣdyn".
+        case : var hvk hk => hvk.
+        - case => [-> | ->] /=.
+          * iDestruct ("hiϕ" $! w) as "[h0 _]"; iClear "hiϕ".
+            rewrite !interp_dynamic_unfold; iApply "h0"; iClear "h0".
+            replace ty with (subst_ty σ (GenT k)); last by rewrite /= htk.
+            rewrite interp_type_subst; last first.
+            { apply lookup_lt_Some in htk.
+              by constructor.
+            }
+            iAssert (Σdyn !! k ≡ Some (interp_type (GenT k) Σdyn))%I as "hϕi".
+            { destruct (Σdyn !! k) as [? | ] eqn:heq.
+              - rewrite !option_equivI.
+                iPureIntro => w'.
+                by rewrite interp_generic_unfold /interp_generic heq /=.
+              - apply lookup_ge_None_1 in heq.
+                apply lookup_lt_Some in htk.
+                rewrite hlen hl0 in heq.
+                apply lt_not_le in htk.
+                by apply htk in heq.
+            }
+            iRewrite "hϕ" in "hϕi".
+            rewrite !option_equivI.
+            iRewrite "hϕi".
+            assert (hmono : mono dyndef.(generics) (GenT k)).
+            { by constructor. }
+            by iApply interp_with_mono.
+          * iDestruct ("hiϕ" $! w) as "[_ h0]"; iClear "hiϕ".
+            replace ty with (subst_ty σ (GenT k)); last by rewrite /= htk.
+            rewrite interp_type_subst; last first.
+            { apply lookup_lt_Some in htk.
+              by constructor.
+            }
+            rewrite !interp_dynamic_unfold.
+            iDestruct ("h0" with "h") as "h1"; iClear "h0 h".
+            iAssert (Σdyn !! k ≡ Some (interp_type (GenT k) Σdyn))%I as "hϕi".
+            { destruct (Σdyn !! k) as [? | ] eqn:heq.
+              - rewrite !option_equivI.
+                iPureIntro => w'.
+                by rewrite interp_generic_unfold /interp_generic heq /=.
+              - apply lookup_ge_None_1 in heq.
+                apply lookup_lt_Some in htk.
+                rewrite hlen hl0 in heq.
+                apply lt_not_le in htk.
+                by apply htk in heq.
+            }
+            iRewrite "hϕ" in "hϕi".
+            rewrite !option_equivI.
+            iRewrite "hϕi" in "h1"; iClear "hϕi".
+            iDestruct (neg_interp_variance with "hf0") as "hf1"; iClear "hf0".
+            assert (hmono : mono (neg_variance <$> dyndef.(generics)) (GenT k)).
+            { constructor.
+              by rewrite list_lookup_fmap hvk.
+            }
+            by iApply interp_with_mono.
+        - move => ->.
+          iSpecialize ("hiϕ" $! w).
+          rewrite /= !interp_dynamic_unfold; iApply "hiϕ".
+          replace ty with (subst_ty σ (GenT k)); last by rewrite /= htk.
+          rewrite interp_type_subst; last first.
+          { apply lookup_lt_Some in htk.
+            by constructor.
+          }
+          iAssert (Σdyn !! k ≡ Some (interp_type (GenT k) Σdyn))%I as "hϕi".
+          { destruct (Σdyn !! k) as [? | ] eqn:heq.
+            - rewrite !option_equivI.
+              iPureIntro => w'.
+              by rewrite interp_generic_unfold /interp_generic heq /=.
+            - apply lookup_ge_None_1 in heq.
+              apply lookup_lt_Some in htk.
+              rewrite hlen hl0 in heq.
+              apply lt_not_le in htk.
+              by apply htk in heq.
+          }
+          iRewrite "hϕ" in "hϕi".
+          rewrite !option_equivI.
+          iRewrite "hϕi".
+          assert (hmono : mono dyndef.(generics) (GenT k)).
+          { by constructor. }
+          by iApply interp_with_mono.
+        - move => ->.
+          iSpecialize ("hiϕ" $! w).
+          replace ty with (subst_ty σ (GenT k)); last by rewrite /= htk.
+          rewrite interp_type_subst; last first.
+          { apply lookup_lt_Some in htk.
+            by constructor.
+          }
+          rewrite !interp_dynamic_unfold.
+          iDestruct ("hiϕ" with "h") as "h1".
+          iAssert (Σdyn !! k ≡ Some (interp_type (GenT k) Σdyn))%I as "hϕi".
+          { destruct (Σdyn !! k) as [? | ] eqn:heq.
+            - rewrite !option_equivI.
+              iPureIntro => w'.
+              by rewrite interp_generic_unfold /interp_generic heq /=.
+            - apply lookup_ge_None_1 in heq.
+              apply lookup_lt_Some in htk.
+              rewrite hlen hl0 in heq.
+              apply lt_not_le in htk.
+              by apply htk in heq.
+          }
+          iRewrite "hϕ" in "hϕi".
+          rewrite !option_equivI.
+          iRewrite "hϕi" in "h1"; iClear "hϕi".
+          iDestruct (neg_interp_variance with "hf0") as "hf1"; iClear "hf0".
+          assert (hmono : mono (neg_variance <$> dyndef.(generics)) (GenT k)).
+          { apply MonoVCoGen.
+            by rewrite list_lookup_fmap hvk.
+          }
+          by iApply interp_with_mono.
+      }
+      iAssert (□ Σinterp Σt (constraints def0 ++ Δdyn))%I as "hconstr_".
+      { iModIntro.
+        by iApply Σinterp_app.
+      }
+      iSpecialize ("hdyn" $! name Public fty orig hf).
       iDestruct "H▷" as "[%hdf h]".
       iRewrite -"HΦ" in "hdyn".
       iSpecialize ("h" $! name _ with "[hdyn]"); first done.
       iDestruct "h" as (w) "[%hw hiw]".
       simplify_eq.
-      iDestruct (subtype_is_inclusion _ hwfc wf_parent wf_mono _ Σt _ _ hsub v) as "hsub".
+      iDestruct (subtype_is_inclusion _ hwf_ wf_parent wf_mono _ Σt _ _ hsub' v) as "hsub".
       { by apply has_field_wf in hf. }
       by iApply "hsub".
     }
